LC/NV/UTLC/Sub/Sub.lean
@@ -415,17 +415,17 @@ example
   (e1 e2 e3 : Term_)
   (v : Symbol_)
   (h1 : is_sub_v0 e1 v e2 e3) :
-  is_sub_v1 e1 v e2 e3 :=
+  is_sub_v2 e1 v e2 e3 :=
   by
     induction h1
     case var_same y x N ih =>
-      apply is_sub_v1.var_same
+      apply is_sub_v2.var_same
       exact ih
     case var_diff y x N ih =>
-      apply is_sub_v1.var_diff
+      apply is_sub_v2.var_diff
       exact ih
     case app P Q x N P' Q' ih_1 ih_2 ih_3 ih_4 =>
-      apply is_sub_v1.app
+      apply is_sub_v2.app
       · exact ih_3
       · exact ih_4
     case abs_diff_nel y P x N ih =>
@@ -433,14 +433,14 @@ example
       simp at ih
       by_cases c1 : x = y
       case pos =>
-        apply is_sub_v1.abs_same
+        apply is_sub_v2.abs_same
         exact c1
       case neg =>
-        apply is_sub_v1.abs_diff_nel
+        apply is_sub_v2.abs_diff_nel
         · exact c1
         · tauto
     case abs_diff y P x N P' ih_1 ih_2 ih_3 ih_4 =>
-      apply is_sub_v1.abs_diff
+      apply is_sub_v2.abs_diff
       · exact ih_1
       · exact ih_2
       · exact ih_4
@@ -449,7 +449,7 @@ example
 example
   (e1 e2 e3 : Term_)
   (v : Symbol_)
-  (h1 : is_sub_v1 e1 v e2 e3) :
+  (h1 : is_sub_v2 e1 v e2 e3) :
   is_sub_v0 e1 v e2 e3 :=
   by
     induction h1
@@ -488,7 +488,7 @@ example
 example
   (e1 e2 e3 : Term_)
   (v : Symbol_)
-  (h1 : is_sub_v1 e1 v e2 e3) :
+  (h1 : is_sub_v2 e1 v e2 e3) :
   is_sub_v3 e1 v e2 e3 :=
   by
     induction h1
@@ -523,7 +523,7 @@ theorem extracted_1
   (v : Symbol_)
   (e2 e3 : Term_)
   (h1: v ∉ e1.free_var_set)
-  (h2 : is_sub_v1 e1 v e2 e3) :
+  (h2 : is_sub_v2 e1 v e2 e3) :
   e1 = e3 :=
   by
     induction h2
@@ -556,21 +556,21 @@ example
   (e1 e2 e3 : Term_)
   (v : Symbol_)
   (h1 : is_sub_v3 e1 v e2 e3) :
-  is_sub_v1 e1 v e2 e3 :=
+  is_sub_v2 e1 v e2 e3 :=
   by
     induction h1
     case var_same y x N ih =>
-      apply is_sub_v1.var_same
+      apply is_sub_v2.var_same
       exact ih
     case var_diff y x N ih =>
-      apply is_sub_v1.var_diff
+      apply is_sub_v2.var_diff
       exact ih
     case app P Q x N P' Q' ih_1 ih_2 ih_3 ih_4 =>
-      apply is_sub_v1.app
+      apply is_sub_v2.app
       · exact ih_3
       · exact ih_4
     case abs_same y P x N ih =>
-      apply is_sub_v1.abs_same
+      apply is_sub_v2.abs_same
       exact ih
     case abs_diff_nel y P x N P' ih_1 ih_2 ih_3 ih_4 =>
       have s1 : x ∉ (abs_ y P).free_var_set :=
@@ -583,11 +583,11 @@ example
       by
         apply extracted_1 P x N P' ih_2 ih_4
       subst s2
-      apply is_sub_v1.abs_diff_nel
+      apply is_sub_v2.abs_diff_nel
       · exact ih_1
       · exact ih_2
     case abs_diff y P x N P' ih_1 ih_2 ih_3 ih_4 =>
-      apply is_sub_v1.abs_diff
+      apply is_sub_v2.abs_diff
       · exact ih_1
       · exact ih_2
       · exact ih_4
